Cook_Levin_IMP/Views/IMP_Minus_Tailcalls/HOL_To_IMP_Minus_Tailcalls_Tactics.thy
@@ -1,0 +1,51 @@
+\<^marker>\<open>creator "Kevin Kappelmann"\<close>
+theory HOL_To_IMP_Minus_Tailcalls_Tactics
+  imports
+    States_Cook_Levin_IMP_Minus_Tailcalls
+    IMP_Minus.Compile_Nat
+begin
+
+unbundle Com.no_com_syntax
+unbundle IMP_Tailcalls_Dynamic.tcom_syntax
+
+lemma tSeq_assoc:
+  "c \<turnstile> (tSeq (tSeq p1 p2) p3, s) \<Rightarrow>\<^bsup>t \<^esup> s' \<longleftrightarrow> c \<turnstile> (tSeq p1 (tSeq p2 p3), s) \<Rightarrow>\<^bsup>t \<^esup> s'"
+  by auto
+
+lemma tAssignD: "c \<turnstile> (x ::= a, s) \<Rightarrow>\<^bsup>t\<^esup> s' \<Longrightarrow> t = 2 \<and> s' = s(x := aval a s)"
+  by auto
+
+ML_file \<open>hol_to_imp_minus_tailcalls_tactics.ML\<close>
+
+ML \<open>
+  structure H = HOL_To_IMP_Minus_Tailcalls_Tactics
+\<close>
+
+lemma Not_IMP_func_correct:
+  includes tcom_syntax
+  assumes "(inline (compile (not_IMP)), s) \<Rightarrow>\<^bsup>t\<^esup> s'"
+  shows "s' ''not_ret'' = not_nat (s ''not_x'')"
+  using assms
+  apply -
+  apply (erule inline)
+  apply (erule compile_complete)
+  apply (simp add: not_IMP_def)
+  (*apply (simp only: set_vars_compile vars_tcom.simps)*)
+  subgoal 
+  apply (tactic \<open>H.start_tac @{thm not_IMP_def} @{context} 1\<close>)
+  apply (tactic \<open>H.seq_tac @{context} 1\<close>)
+  apply (tactic \<open>H.assign_tac @{context} 1\<close>)
+  apply (tactic \<open>H.seq_tac @{context} 1\<close>)
+  apply (tactic \<open>H.assign_tac @{context} 1\<close>)
+  apply (tactic \<open>H.seq_tac @{context} 1\<close>)
+  apply (tactic \<open>H.assign_tac @{context} 1\<close>)
+  apply (tactic \<open>H.seq_tac @{context} 1\<close>)
+  apply (tactic \<open>H.call_tac @{thm eq_IMP_func_correct} @{thm refl} @{context} 1\<close>)
+  apply (tactic \<open>H.seq_tac @{context} 1\<close>)
+  apply (tactic \<open>H.assign_tac @{context} 1\<close>)
+  apply (tactic \<open>H.assign_tac @{context} 1\<close>)
+  sorry
+  done
+
+
+end
