IMP-/IMP_Tailcalls_Dynamic.thy
@@ -29,16 +29,16 @@ unbundle no_com'_syntax
 unbundle tcom_syntax
 
 inductive
-  tbig_step_t :: "tcom \<Rightarrow> tcom \<times> state \<Rightarrow> nat \<Rightarrow> state \<Rightarrow> bool" ("_ \<turnstile>_ \<Rightarrow>\<^bsup> _\<^esup>  _" 55)
+  tbig_step_t :: "tcom \<Rightarrow> tcom \<times> state \<Rightarrow> nat \<Rightarrow> state \<Rightarrow> bool" ("_ \<turnstile>_ \<Rightarrow>\<^bsup>_\<^esup>  _" 55)
 where
-tSkip: "c \<turnstile> (tSKIP,s) \<Rightarrow>\<^bsup> Suc (0::nat) \<^esup> s" |
-tAssign: "c \<turnstile>(x ::= a,s) \<Rightarrow>\<^bsup> Suc (Suc 0) \<^esup> s(x := aval a s)" |
-tSeq: "\<lbrakk>c \<turnstile> (c1,s1) \<Rightarrow>\<^bsup> x \<^esup> s2; c \<turnstile> (c2,s2) \<Rightarrow>\<^bsup> y \<^esup> s3 ; z=x+y \<rbrakk> \<Longrightarrow> c \<turnstile> (c1;;c2, s1) \<Rightarrow>\<^bsup> z \<^esup> s3" |
-tIfTrue: "\<lbrakk> s b \<noteq> 0;  c \<turnstile> (c1,s) \<Rightarrow>\<^bsup> x \<^esup> t; y=x+1 \<rbrakk> \<Longrightarrow> c \<turnstile> (IF b \<noteq>0 THEN c1 ELSE c2, s) \<Rightarrow>\<^bsup> y \<^esup> t" |
-tIfFalse: "\<lbrakk> s b = 0; c \<turnstile> (c2,s) \<Rightarrow>\<^bsup> x \<^esup> t; y=x+1  \<rbrakk> \<Longrightarrow> c \<turnstile> (IF b \<noteq>0 THEN c1 ELSE c2, s) \<Rightarrow>\<^bsup> y \<^esup> t" |
-tCall: "(C,s) \<Rightarrow>\<^bsup> z \<^esup> t \<Longrightarrow> c \<turnstile> (CALL C RETURN r,s) \<Rightarrow>\<^bsup> z \<^esup> (s(r:=t r))" |
+tSkip: "c \<turnstile> (tSKIP,s) \<Rightarrow>\<^bsup>Suc (0::nat) \<^esup> s" |
+tAssign: "c \<turnstile>(x ::= a,s) \<Rightarrow>\<^bsup>Suc (Suc 0) \<^esup> s(x := aval a s)" |
+tSeq: "\<lbrakk>c \<turnstile> (c1,s1) \<Rightarrow>\<^bsup>x \<^esup> s2; c \<turnstile> (c2,s2) \<Rightarrow>\<^bsup>y \<^esup> s3 ; z=x+y \<rbrakk> \<Longrightarrow> c \<turnstile> (c1;;c2, s1) \<Rightarrow>\<^bsup>z \<^esup> s3" |
+tIfTrue: "\<lbrakk> s b \<noteq> 0;  c \<turnstile> (c1,s) \<Rightarrow>\<^bsup>x \<^esup> t; y=x+1 \<rbrakk> \<Longrightarrow> c \<turnstile> (IF b \<noteq>0 THEN c1 ELSE c2, s) \<Rightarrow>\<^bsup>y \<^esup> t" |
+tIfFalse: "\<lbrakk> s b = 0; c \<turnstile> (c2,s) \<Rightarrow>\<^bsup>x \<^esup> t; y=x+1  \<rbrakk> \<Longrightarrow> c \<turnstile> (IF b \<noteq>0 THEN c1 ELSE c2, s) \<Rightarrow>\<^bsup>y \<^esup> t" |
+tCall: "(C,s) \<Rightarrow>\<^bsup>z \<^esup> t \<Longrightarrow> c \<turnstile> (CALL C RETURN r,s) \<Rightarrow>\<^bsup>z \<^esup> (s(r:=t r))" |
 \<comment> \<open>New rule\<close>
-tTail: "c \<turnstile> (c,s) \<Rightarrow>\<^bsup> z \<^esup> t \<Longrightarrow> c \<turnstile> (tTAIL,s) \<Rightarrow>\<^bsup> 5 + z \<^esup> t"
+tTail: "c \<turnstile> (c,s) \<Rightarrow>\<^bsup>z \<^esup> t \<Longrightarrow> c \<turnstile> (tTAIL,s) \<Rightarrow>\<^bsup>5 + z \<^esup> t"
 
 code_pred tbig_step_t .
 
@@ -47,13 +47,13 @@ declare tbig_step_t.intros[intro]
 lemmas tbig_step_t_induct = tbig_step_t.induct[split_format(complete)]
 
 
-inductive_cases tSkip_tE[elim!]: "c \<turnstile> (tSKIP,s) \<Rightarrow>\<^bsup> x \<^esup> t"
-inductive_cases tAssign_tE[elim!]: "c \<turnstile> (x ::= a,s) \<Rightarrow>\<^bsup> p \<^esup> t"
-inductive_cases tSeq_tE[elim!]: "c \<turnstile> (c1;;c2,s1) \<Rightarrow>\<^bsup> p \<^esup> s3"
-inductive_cases tIf_tE[elim!]: "c \<turnstile> (IF b \<noteq>0 THEN c1 ELSE c2,s) \<Rightarrow>\<^bsup> x \<^esup> t"
-inductive_cases tCall_tE[elim!]: "c \<turnstile> (CALL C RETURN v,s) \<Rightarrow>\<^bsup> z \<^esup> t"
+inductive_cases tSkip_tE[elim!]: "c \<turnstile> (tSKIP,s) \<Rightarrow>\<^bsup>x \<^esup> t"
+inductive_cases tAssign_tE[elim!]: "c \<turnstile> (x ::= a,s) \<Rightarrow>\<^bsup>p \<^esup> t"
+inductive_cases tSeq_tE[elim!]: "c \<turnstile> (c1;;c2,s1) \<Rightarrow>\<^bsup>p \<^esup> s3"
+inductive_cases tIf_tE[elim!]: "c \<turnstile> (IF b \<noteq>0 THEN c1 ELSE c2,s) \<Rightarrow>\<^bsup>x \<^esup> t"
+inductive_cases tCall_tE[elim!]: "c \<turnstile> (CALL C RETURN v,s) \<Rightarrow>\<^bsup>z \<^esup> t"
 
-inductive_cases tTail_tE[elim]: "c \<turnstile> (tTAIL,s) \<Rightarrow>\<^bsup> x \<^esup> t"
+inductive_cases tTail_tE[elim]: "c \<turnstile> (tTAIL,s) \<Rightarrow>\<^bsup>x \<^esup> t"
 
 
 instantiation tcom :: vars
@@ -87,15 +87,15 @@ lemma no_tails_invar[simp]: "\<not>tails c \<Longrightarrow> invar c"
 
 section \<open>Semantics for small-step-ish reasoning (loops)\<close>
 inductive
-  tail_step :: "(tcom \<times> state) \<Rightarrow> nat \<Rightarrow> (state \<times> bool) \<Rightarrow> bool" ("\<turnstile>_ \<Rightarrow>\<^bsup> _\<^esup>  _" 55)
+  tail_step :: "(tcom \<times> state) \<Rightarrow> nat \<Rightarrow> (state \<times> bool) \<Rightarrow> bool" ("\<turnstile>_ \<Rightarrow>\<^bsup>_\<^esup>  _" 55)
 where
-Skip: "\<turnstile> (tSKIP,s) \<Rightarrow>\<^bsup> Suc (0::nat) \<^esup> (s,False)" |
-Assign: "\<turnstile>(x ::= a,s) \<Rightarrow>\<^bsup> Suc (Suc 0) \<^esup> (s(x := aval a s),False)" |
-Seq: "\<lbrakk>\<turnstile> (c1,s1) \<Rightarrow>\<^bsup> x \<^esup> (s2, False); \<turnstile> (c2,s2) \<Rightarrow>\<^bsup> y \<^esup> (s3,CONT) ; z=x+y \<rbrakk> \<Longrightarrow> \<turnstile> (c1;;c2, s1) \<Rightarrow>\<^bsup> z \<^esup> (s3,CONT)" |
-IfTrue: "\<lbrakk> s b \<noteq> 0;  \<turnstile> (c1,s) \<Rightarrow>\<^bsup> x \<^esup> (t,CONT); y=x+1 \<rbrakk> \<Longrightarrow> \<turnstile> (IF b \<noteq>0 THEN c1 ELSE c2, s) \<Rightarrow>\<^bsup> y \<^esup> (t,CONT)" |
-IfFalse: "\<lbrakk> s b = 0; \<turnstile> (c2,s) \<Rightarrow>\<^bsup> x \<^esup> (t,CONT); y=x+1  \<rbrakk> \<Longrightarrow> \<turnstile> (IF b \<noteq>0 THEN c1 ELSE c2, s) \<Rightarrow>\<^bsup> y \<^esup> (t,CONT)" |
-Call: "(C,s) \<Rightarrow>\<^bsup> z \<^esup> t \<Longrightarrow> \<turnstile> (CALL C RETURN r,s) \<Rightarrow>\<^bsup> z \<^esup> (s(r:=t r),False)" |
-Tail: "\<turnstile> (tTAIL,s) \<Rightarrow>\<^bsup> 5 \<^esup> (s,True)"
+Skip: "\<turnstile> (tSKIP,s) \<Rightarrow>\<^bsup>Suc (0::nat) \<^esup> (s,False)" |
+Assign: "\<turnstile>(x ::= a,s) \<Rightarrow>\<^bsup>Suc (Suc 0) \<^esup> (s(x := aval a s),False)" |
+Seq: "\<lbrakk>\<turnstile> (c1,s1) \<Rightarrow>\<^bsup>x \<^esup> (s2, False); \<turnstile> (c2,s2) \<Rightarrow>\<^bsup>y \<^esup> (s3,CONT) ; z=x+y \<rbrakk> \<Longrightarrow> \<turnstile> (c1;;c2, s1) \<Rightarrow>\<^bsup>z \<^esup> (s3,CONT)" |
+IfTrue: "\<lbrakk> s b \<noteq> 0;  \<turnstile> (c1,s) \<Rightarrow>\<^bsup>x \<^esup> (t,CONT); y=x+1 \<rbrakk> \<Longrightarrow> \<turnstile> (IF b \<noteq>0 THEN c1 ELSE c2, s) \<Rightarrow>\<^bsup>y \<^esup> (t,CONT)" |
+IfFalse: "\<lbrakk> s b = 0; \<turnstile> (c2,s) \<Rightarrow>\<^bsup>x \<^esup> (t,CONT); y=x+1  \<rbrakk> \<Longrightarrow> \<turnstile> (IF b \<noteq>0 THEN c1 ELSE c2, s) \<Rightarrow>\<^bsup>y \<^esup> (t,CONT)" |
+Call: "(C,s) \<Rightarrow>\<^bsup>z \<^esup> t \<Longrightarrow> \<turnstile> (CALL C RETURN r,s) \<Rightarrow>\<^bsup>z \<^esup> (s(r:=t r),False)" |
+Tail: "\<turnstile> (tTAIL,s) \<Rightarrow>\<^bsup>5 \<^esup> (s,True)"
 
 code_pred tail_step .
 
@@ -103,19 +103,19 @@ declare tail_step.intros[intro]
 
 lemmas tail_step_induct = tail_step.induct[split_format(complete)]
 
-inductive_cases tailSkip_tE[elim!]: "\<turnstile> (tSKIP,s) \<Rightarrow>\<^bsup> x \<^esup> (t,b)"
-inductive_cases tailAssign_tE[elim!]: "\<turnstile> (x ::= a,s) \<Rightarrow>\<^bsup> p \<^esup> (t,b)"
-inductive_cases tailSeq_tE[elim!]: "\<turnstile> (c1;;c2,s1) \<Rightarrow>\<^bsup> p \<^esup> (s3,b)"
-inductive_cases tailIf_tE[elim!]: "\<turnstile> (IF b \<noteq>0 THEN c1 ELSE c2,s) \<Rightarrow>\<^bsup> x \<^esup> (t,CONT)"
-inductive_cases tailCall_tE[elim!]: "\<turnstile> (CALL C RETURN v,s) \<Rightarrow>\<^bsup> z \<^esup> (t,b)"
+inductive_cases tailSkip_tE[elim!]: "\<turnstile> (tSKIP,s) \<Rightarrow>\<^bsup>x \<^esup> (t,b)"
+inductive_cases tailAssign_tE[elim!]: "\<turnstile> (x ::= a,s) \<Rightarrow>\<^bsup>p \<^esup> (t,b)"
+inductive_cases tailSeq_tE[elim!]: "\<turnstile> (c1;;c2,s1) \<Rightarrow>\<^bsup>p \<^esup> (s3,b)"
+inductive_cases tailIf_tE[elim!]: "\<turnstile> (IF b \<noteq>0 THEN c1 ELSE c2,s) \<Rightarrow>\<^bsup>x \<^esup> (t,CONT)"
+inductive_cases tailCall_tE[elim!]: "\<turnstile> (CALL C RETURN v,s) \<Rightarrow>\<^bsup>z \<^esup> (t,b)"
 
-inductive_cases tailTail_tE[elim]: "\<turnstile> (tTAIL,s) \<Rightarrow>\<^bsup> x \<^esup> (t,b)"
+inductive_cases tailTail_tE[elim]: "\<turnstile> (tTAIL,s) \<Rightarrow>\<^bsup>x \<^esup> (t,b)"
 
 inductive
-  tail_steps :: "tcom \<Rightarrow> tcom \<times> state \<Rightarrow> nat \<Rightarrow> state \<Rightarrow> bool" ("_ \<turnstile>''_ \<Rightarrow>\<^bsup> _\<^esup>  _" 55) for d
+  tail_steps :: "tcom \<Rightarrow> tcom \<times> state \<Rightarrow> nat \<Rightarrow> state \<Rightarrow> bool" ("_ \<turnstile>''_ \<Rightarrow>\<^bsup>_\<^esup>  _" 55) for d
 where
-tFalse: "\<turnstile>(c,s) \<Rightarrow>\<^bsup> z \<^esup> (t,False) \<Longrightarrow> d \<turnstile>'(c,s)\<Rightarrow>\<^bsup> z \<^esup> t" |
-tTrue: "\<turnstile>(c,s1) \<Rightarrow>\<^bsup> x \<^esup> (s2,True) \<Longrightarrow> d \<turnstile>'(d,s2)\<Rightarrow>\<^bsup> y \<^esup> s3 \<Longrightarrow> d \<turnstile>'(c,s1)\<Rightarrow>\<^bsup> x+y \<^esup> s3"
+tFalse: "\<turnstile>(c,s) \<Rightarrow>\<^bsup>z \<^esup> (t,False) \<Longrightarrow> d \<turnstile>'(c,s)\<Rightarrow>\<^bsup>z \<^esup> t" |
+tTrue: "\<turnstile>(c,s1) \<Rightarrow>\<^bsup>x \<^esup> (s2,True) \<Longrightarrow> d \<turnstile>'(d,s2)\<Rightarrow>\<^bsup>y \<^esup> s3 \<Longrightarrow> d \<turnstile>'(c,s1)\<Rightarrow>\<^bsup>x+y \<^esup> s3"
 
 code_pred tail_steps .
 
@@ -124,16 +124,16 @@ declare tail_steps.cases[elim]
 
 lemmas tail_steps_induct = tail_steps.induct[split_format(complete)]
 
-lemma no_tails_no_step: "\<turnstile>(c,s) \<Rightarrow>\<^bsup> z \<^esup> (t,b) \<Longrightarrow> \<not>tails c \<Longrightarrow> \<not>b"
+lemma no_tails_no_step: "\<turnstile>(c,s) \<Rightarrow>\<^bsup>z \<^esup> (t,b) \<Longrightarrow> \<not>tails c \<Longrightarrow> \<not>b"
   by (induction c s z t b rule: tail_step_induct) auto
 
-lemma no_tails_sem: "\<turnstile>(c,s) \<Rightarrow>\<^bsup> z \<^esup> (t,b) \<Longrightarrow> \<not>tails c \<Longrightarrow> d \<turnstile> (c,s)\<Rightarrow>\<^bsup> z \<^esup> t"
+lemma no_tails_sem: "\<turnstile>(c,s) \<Rightarrow>\<^bsup>z \<^esup> (t,b) \<Longrightarrow> \<not>tails c \<Longrightarrow> d \<turnstile> (c,s)\<Rightarrow>\<^bsup>z \<^esup> t"
   by (induction c s z t b rule: tail_step_induct) auto
 
-lemma small_sound: "d \<turnstile> (c,s) \<Rightarrow>\<^bsup> z \<^esup> t \<Longrightarrow> invar c \<Longrightarrow> invar d \<Longrightarrow> d \<turnstile>' (c,s) \<Rightarrow>\<^bsup> z \<^esup> t"
+lemma small_sound: "d \<turnstile> (c,s) \<Rightarrow>\<^bsup>z \<^esup> t \<Longrightarrow> invar c \<Longrightarrow> invar d \<Longrightarrow> d \<turnstile>' (c,s) \<Rightarrow>\<^bsup>z \<^esup> t"
 proof (induction d c s z t rule: tbig_step_t_induct)
   case (tSeq c c1 s1 x s2 c2 y s3 z)
-  hence "c \<turnstile>'(c1, s1) \<Rightarrow>\<^bsup> x\<^esup>  s2" "c \<turnstile>'(c2, s2) \<Rightarrow>\<^bsup> y\<^esup>  s3" by auto
+  hence "c \<turnstile>'(c1, s1) \<Rightarrow>\<^bsup>x\<^esup>  s2" "c \<turnstile>'(c2, s2) \<Rightarrow>\<^bsup>y\<^esup>  s3" by auto
   from this tSeq show ?case apply (cases) apply auto
     subgoal
       by (smt (verit) ab_semigroup_add_class.add_ac(1) tail_step.Seq tail_steps.simps)
@@ -142,23 +142,23 @@ proof (induction d c s z t rule: tbig_step_t_induct)
     done
 next
   case (tIfTrue s b c c1 x t y c2)
-  hence "c \<turnstile>'(c1, s) \<Rightarrow>\<^bsup> x\<^esup>  t" by auto
+  hence "c \<turnstile>'(c1, s) \<Rightarrow>\<^bsup>x\<^esup>  t" by auto
   from this tIfTrue show ?case apply (cases) apply auto apply force
     by (metis Suc_eq_plus1 local.tIfTrue(1) plus_nat.simps(2) tail_step.IfTrue tail_steps.intros(2))
 next
   case (tIfFalse s b c c2 x t y c1)
-  hence "c \<turnstile>'(c2, s) \<Rightarrow>\<^bsup> x\<^esup>  t" by auto
+  hence "c \<turnstile>'(c2, s) \<Rightarrow>\<^bsup>x\<^esup>  t" by auto
   from this tIfFalse show ?case apply (cases) apply auto apply force
     by (metis Suc_eq_plus1 add_Suc tTrue tail_step.IfFalse)
 next
   case (tTail c s z t)
-  hence " c \<turnstile>'(c, s) \<Rightarrow>\<^bsup> z\<^esup>  t" by simp
-  moreover have "\<turnstile>(tTAIL,s) \<Rightarrow>\<^bsup> 5 \<^esup> (s,True)"
+  hence " c \<turnstile>'(c, s) \<Rightarrow>\<^bsup>z\<^esup>  t" by simp
+  moreover have "\<turnstile>(tTAIL,s) \<Rightarrow>\<^bsup>5 \<^esup> (s,True)"
     by (metis Tail)
   ultimately show ?case by auto
 qed auto
 
-lemma small_complete: "d \<turnstile>' (c,s) \<Rightarrow>\<^bsup> z \<^esup> t \<Longrightarrow> invar c \<Longrightarrow> invar d \<Longrightarrow> d \<turnstile> (c,s) \<Rightarrow>\<^bsup> z \<^esup> t"
+lemma small_complete: "d \<turnstile>' (c,s) \<Rightarrow>\<^bsup>z \<^esup> t \<Longrightarrow> invar c \<Longrightarrow> invar d \<Longrightarrow> d \<turnstile> (c,s) \<Rightarrow>\<^bsup>z \<^esup> t"
 proof (induction c s z t rule: tail_steps_induct)
   case (tFalse c s z t)
   then show ?case
@@ -168,7 +168,7 @@ next
   then show ?case
   proof (induction c s1 x s2 True arbitrary:  rule: tail_step_induct)
     case (Seq c1 s1 x s2 c2 y s3 z)
-    then show ?case using no_tails_sem apply auto 
+    then show ?case using no_tails_sem apply auto
       using ab_semigroup_add_class.add_ac(1) by blast
   qed auto
 qed
@@ -182,38 +182,38 @@ lemma while'_unrolling:
   shows "(c;;WHILE b\<noteq>0 DO c,s)\<Rightarrow>'\<^bsup>z\<^esup> t = (WHILE b\<noteq>0 DO c,s)\<Rightarrow>'\<^bsup>1+z\<^esup> t"
   using assms by auto
 
-lemma tnoninterference: 
-  "\<lbrakk>c'\<turnstile>(c,s) \<Rightarrow>\<^bsup> x \<^esup> t; set (vars c) \<subseteq> S; set (vars c') \<subseteq> S; v \<notin> S \<rbrakk> \<Longrightarrow> c'\<turnstile>(c,s(v:=y)) \<Rightarrow>\<^bsup> x \<^esup> t(v:=y)"
+lemma tnoninterference:
+  "\<lbrakk>c'\<turnstile>(c,s) \<Rightarrow>\<^bsup>x \<^esup> t; set (vars c) \<subseteq> S; set (vars c') \<subseteq> S; v \<notin> S \<rbrakk> \<Longrightarrow> c'\<turnstile>(c,s(v:=y)) \<Rightarrow>\<^bsup>x \<^esup> t(v:=y)"
 proof (induction c' c s x t rule: tbig_step_t_induct)
   case (tAssign c x a s)
   hence " s(v := y, x := aval a (s(v := y))) = s(x := aval a s, v := y)" by force
   thus ?case using tbig_step_t.tAssign[of c x a "s(v:=y)"] by argo
 next
   case (tCall C s z t c r)
-  hence Call: "(C, s(v := y)) \<Rightarrow>\<^bsup> z \<^esup> t(v := y)" using fresh_var_changed by fastforce
+  hence Call: "(C, s(v := y)) \<Rightarrow>\<^bsup>z \<^esup> t(v := y)" using fresh_var_changed by fastforce
   from tCall have state: " s(v := y, r := (t(v := y)) r) = s(r := t r, v := y)" by auto
   show ?case using tbig_step_t.tCall[OF Call, of c r] state by argo
 qed (auto | force)+
 
 lemma noninterference':
-  "\<lbrakk>\<turnstile>(c,s) \<Rightarrow>\<^bsup> x \<^esup> (t,b); set (vars c) \<subseteq> S; set (vars c') \<subseteq> S; v \<notin> S \<rbrakk> \<Longrightarrow> \<turnstile>(c,s(v:=y)) \<Rightarrow>\<^bsup> x \<^esup> (t(v:=y),b)"
+  "\<lbrakk>\<turnstile>(c,s) \<Rightarrow>\<^bsup>x \<^esup> (t,b); set (vars c) \<subseteq> S; set (vars c') \<subseteq> S; v \<notin> S \<rbrakk> \<Longrightarrow> \<turnstile>(c,s(v:=y)) \<Rightarrow>\<^bsup>x \<^esup> (t(v:=y),b)"
 proof (induction c s x t b rule: tail_step_induct)
   case (Assign x a s)
   hence "s(v := y, x := aval a (s(v := y))) = s(x := aval a s, v := y)" by force
   then show ?case using tail_step.Assign[of x a "s(v:=y)"] by argo
 next
   case (Call C s z t r)
-   hence Call: "(C, s(v := y)) \<Rightarrow>\<^bsup> z \<^esup> t(v := y)" using fresh_var_changed by fastforce
+   hence Call: "(C, s(v := y)) \<Rightarrow>\<^bsup>z \<^esup> t(v := y)" using fresh_var_changed by fastforce
    from tCall have state: " s(v := y, r := (t(v := y)) r) = s(r := t r, v := y)" by auto
    show ?case using tbig_step_t.tCall[OF Call, of c r] state
      by (metis local.Call tail_step.Call)
 qed auto
 
 lemma tnoninterference':
-  "\<lbrakk>c'\<turnstile>'(c,s) \<Rightarrow>\<^bsup> x \<^esup> t; set (vars c) \<subseteq> S; set (vars c') \<subseteq> S; v \<notin> S \<rbrakk> \<Longrightarrow> c'\<turnstile>'(c,s(v:=y)) \<Rightarrow>\<^bsup> x \<^esup> t(v:=y)"
+  "\<lbrakk>c'\<turnstile>'(c,s) \<Rightarrow>\<^bsup>x \<^esup> t; set (vars c) \<subseteq> S; set (vars c') \<subseteq> S; v \<notin> S \<rbrakk> \<Longrightarrow> c'\<turnstile>'(c,s(v:=y)) \<Rightarrow>\<^bsup>x \<^esup> t(v:=y)"
 proof (induction c s x t rule: tail_steps_induct)
   case (tFalse c s z t)
-  then show ?case 
+  then show ?case
     using noninterference' by blast
 next
   case (tTrue c s1 x s2 y s3)
@@ -266,7 +266,7 @@ next
   then show ?case apply (cases c) using tIfTrue by auto
 next
   case (IfFalse' s b c2 x t y c1)
-  then show ?case apply (cases c) apply auto 
+  then show ?case apply (cases c) apply auto
     using Suc_eq_plus1 by blast
 next
   case (WhileFalse' s b c)
@@ -279,7 +279,7 @@ next
   then show ?case by (cases c) auto
 qed
 
-lemma no_tail_complete: 
+lemma no_tail_complete:
   assumes sem: "(translate1 CONT c;;translate CONT c',s)\<Rightarrow>'\<^bsup>2+z\<^esup>t"
       and no_tail: "\<not>tails c"
       and fresh: "CONT \<notin> set (vars c)"
@@ -294,24 +294,24 @@ proof -
 qed
 
 lemma translate_sound_gen:
-  "\<lbrakk> c' \<turnstile> (c,s) \<Rightarrow>\<^bsup>z\<^esup> t; invar c; invar c'; s CONT = 0; CONT \<notin> S; set (vars c) \<subseteq> S; set (vars c') \<subseteq> S\<rbrakk> 
+  "\<lbrakk> c' \<turnstile> (c,s) \<Rightarrow>\<^bsup>z\<^esup> t; invar c; invar c'; s CONT = 0; CONT \<notin> S; set (vars c) \<subseteq> S; set (vars c') \<subseteq> S\<rbrakk>
      \<Longrightarrow> (translate1 CONT c;;translate CONT c',s) \<Rightarrow>'\<^bsup>Suc(Suc 0)+z\<^esup> t"
 proof (induction c' c s z t rule: tbig_step_t_induct)
   case (tAssign c x a s)
-  then show ?case by (auto simp: translate_def simp del: fun_upd_apply) fastforce 
+  then show ?case by (auto simp: translate_def simp del: fun_upd_apply) fastforce
 next
   case (tSeq c c1 s1 x s2 c2 y s3 z)
   hence 1: "(translate1 CONT c1;; translate CONT c, s1) \<Rightarrow>'\<^bsup> Suc (Suc 0) + x\<^esup>  s2" by auto
 
   from 1 obtain s' x' y' where *:
-    "(translate1 CONT c1, s1)\<Rightarrow>'\<^bsup> x'\<^esup>  s'" 
-    "(translate CONT c, s')\<Rightarrow>'\<^bsup> y'\<^esup> s2" 
+    "(translate1 CONT c1, s1)\<Rightarrow>'\<^bsup> x'\<^esup>  s'"
+    "(translate CONT c, s')\<Rightarrow>'\<^bsup> y'\<^esup> s2"
     "x' + y' = Suc (Suc 0) + x" by auto
   from * have s': "s' CONT = 0" using no_tail_cont1 using tSeq by auto (metis in_mono)
-  with * have 11: "(translate1 CONT c1, s1) \<Rightarrow>'\<^bsup> x\<^esup>  s2" 
+  with * have 11: "(translate1 CONT c1, s1) \<Rightarrow>'\<^bsup> x\<^esup>  s2"
     using translate_def by auto
 
-  from s' * have "s2 CONT = 0" 
+  from s' * have "s2 CONT = 0"
     using tSeq by auto (metis "11" determ)
   with tSeq have 2: "(translate1 CONT c2;; translate CONT c, s2) \<Rightarrow>'\<^bsup> Suc (Suc 0) + y\<^esup>  s3"
     by auto
@@ -321,7 +321,7 @@ next
 
   then show ?case by auto
 next
-  case (tCall C s z t c r)                                    
+  case (tCall C s z t c r)
   then show ?case by (auto simp: translate_def simp del: fun_upd_apply) fastforce
 next
   case (tTail c s z t)
@@ -330,7 +330,7 @@ next
   proof - (* wtf why is this not automatic *)
     have "(CONT ::= A (N 0),s(CONT:=1)) \<Rightarrow>'\<^bsup> 2\<^esup> s(CONT := 0)"
       using Assign'[of CONT "A (N 0)" "s(CONT:=1)"] by (auto simp: eval_nat_numeral)
-    moreover from \<open>s CONT = 0\<close> have "s(CONT := 0) = s" by auto 
+    moreover from \<open>s CONT = 0\<close> have "s(CONT := 0) = s" by auto
     ultimately show ?thesis by simp
   qed
   ultimately have "((CONT ::= A (N 0);;translate1 CONT c);; translate CONT c, s(CONT:=1)) \<Rightarrow>'\<^bsup> 4 + z\<^esup>  t"
@@ -358,10 +358,10 @@ proof -
   ultimately have "((CONT::=A (N 0);;translate1 CONT c);; translate CONT c, s) \<Rightarrow>'\<^bsup> 4+z\<^esup> t(CONT := 0)"
     apply (simp add: numeral_eq_Suc)
     by (smt (verit, ccfv_SIG) Seq'_tE add.assoc add_2_eq_Suc big_step_t'.Seq' numeral_2_eq_2)
-  then show "(translate CONT c,s) \<Rightarrow>'\<^bsup>5+z\<^esup> t(CONT := 0)" using while'_unrolling start translate_def by auto  
+  then show "(translate CONT c,s) \<Rightarrow>'\<^bsup>5+z\<^esup> t(CONT := 0)" using while'_unrolling start translate_def by auto
 qed
 
-lemma translate1_complete: 
+lemma translate1_complete:
   "\<lbrakk> (translate1 CONT c,s)\<Rightarrow>'\<^bsup>z\<^esup>t; s CONT = 0; invar c; set (vars c) \<subseteq> S; CONT \<notin> S \<rbrakk>
      \<Longrightarrow> (if t CONT \<noteq> 0 then \<turnstile>(c,s) \<Rightarrow>\<^bsup>3+z\<^esup> (t(CONT := s CONT),True) else \<turnstile>(c,s) \<Rightarrow>\<^bsup>z\<^esup> (t,False))"
 proof (induction "translate1 CONT c" s z t arbitrary: c rule: big_step_t'_induct)
@@ -375,7 +375,7 @@ next
   case (Seq' c1 s1 x s2 c2 y s3 z)
   then show ?case
     apply (cases c)
-         apply (auto split: if_splits) 
+         apply (auto split: if_splits)
     subgoal
       by (smt (verit, best) Seq'.hyps(2) add.left_commute no_tails_invar no_tails_no_step tail_step.Seq)
     subgoal
@@ -414,18 +414,18 @@ lemma loop_min: "(WHILE b\<noteq>0 DO c, s) \<Rightarrow>'\<^bsup> z\<^esup>  t 
   apply (induction "WHILE b\<noteq>0 DO c" s z t rule: big_step_t'_induct) apply simp using determ by fastforce
 
 lemma translate_complete:
-  "\<lbrakk> (translate CONT c,s)\<Rightarrow>'\<^bsup>5+z\<^esup>t; s CONT \<noteq> 0; invar c; CONT \<notin> set (vars c) \<rbrakk> 
+  "\<lbrakk> (translate CONT c,s)\<Rightarrow>'\<^bsup>5+z\<^esup>t; s CONT \<noteq> 0; invar c; CONT \<notin> set (vars c) \<rbrakk>
     \<Longrightarrow> c \<turnstile>'(c,s) \<Rightarrow>\<^bsup>z\<^esup> t(CONT:= s CONT)"
 proof (induction "translate CONT c" s "5+z" t arbitrary: z rule: big_step_t'_induct)
   case (WhileTrue' s1 b c' x s2 y s3 )
 
   hence c'_def: "c' = CONT::=A (N 0);;translate1 CONT c" and b_def: "b = CONT" by (auto simp: translate_def)
-  
+
   have 0: "(CONT::=A (N 0),s1) \<Rightarrow>'\<^bsup>Suc (Suc 0)\<^esup>s1(CONT := 0)"
     using Assign'[of CONT "A (N 0)" s1,simplified] by (simp add: numeral_eq_Suc)
-  
+
   obtain x' where 1:
-    "x' + Suc (Suc 0) = x" "(translate1 CONT c,s1(CONT:=0))\<Rightarrow>'\<^bsup> x'\<^esup>s2" 
+    "x' + Suc (Suc 0) = x" "(translate1 CONT c,s1(CONT:=0))\<Rightarrow>'\<^bsup> x'\<^esup>s2"
     using WhileTrue'.hyps (2)[unfolded c'_def] by auto
 
   show ?case proof (cases "s2 CONT = 0")
@@ -436,23 +436,23 @@ proof (induction "translate CONT c" s "5+z" t arbitrary: z rule: big_step_t'_ind
     ultimately have "\<turnstile>(c,s1) \<Rightarrow>\<^bsup>x'\<^esup> (s3(CONT := s1 CONT),False)"
       using WhileTrue' noninterference'
       by (smt (verit, ccfv_threshold) fun_upd_idem_iff fun_upd_upd order_le_less)
-    hence "c \<turnstile>'(c, s1) \<Rightarrow>\<^bsup> x'\<^esup>  s3(CONT := s1 CONT)" by auto
+    hence "c \<turnstile>'(c, s1) \<Rightarrow>\<^bsup>x'\<^esup>  s3(CONT := s1 CONT)" by auto
     moreover from  \<open>x' + Suc (Suc 0) = x\<close> \<open>1 + x + y = 5+z\<close> \<open>y = Suc (Suc 0)\<close> have "x' = z" by simp
     ultimately show ?thesis by blast
   next
     case False
     with \<open>(WHILE b\<noteq>0 DO c', s2) \<Rightarrow>'\<^bsup> y\<^esup>  s3\<close> obtain s2' z' where "(c',s2) \<Rightarrow>'\<^bsup>z'\<^esup> s2'"
-      using b_def by auto 
+      using b_def by auto
     hence "z' \<ge> 2" unfolding c'_def by auto
-    with loop_min have "y \<ge> 5" 
+    with loop_min have "y \<ge> 5"
       using False WhileTrue'.hyps(4) \<open>(c', s2) \<Rightarrow>'\<^bsup> z'\<^esup> s2'\<close> b_def by fastforce
-    then obtain y' where y'_def: "y = 5 + y'" 
+    then obtain y' where y'_def: "y = 5 + y'"
       using nat_le_iff_add by blast
     from 1 have 2: "\<turnstile>(c,s1(CONT:=0)) \<Rightarrow>\<^bsup>1+x\<^esup> (s2(CONT := 0), True)"
       using translate1_complete[of CONT c "s1(CONT := 0)" x' s2] False WhileTrue' by (auto simp: numeral_eq_Suc)
 
     from False WhileTrue' y'_def have "c \<turnstile>'(c, s2) \<Rightarrow>\<^bsup>y'\<^esup>  s3(CONT := s2 CONT)" by auto
-    hence 3: "c \<turnstile>'(c, s2(CONT := 0)) \<Rightarrow>\<^bsup> y'\<^esup>  s3(CONT := 0)"
+    hence 3: "c \<turnstile>'(c, s2(CONT := 0)) \<Rightarrow>\<^bsup>y'\<^esup>  s3(CONT := 0)"
       using tnoninterference' WhileTrue' by (metis fun_upd_upd order.refl)
 
     from \<open>1 + x + y = 5 + z\<close> y'_def have "c \<turnstile>'(c, s1(CONT := 0)) \<Rightarrow>\<^bsup>z\<^esup>  s3(CONT := 0)"
@@ -482,20 +482,20 @@ proof -
     using Assign'[of ?CONT "A (N 1)" s] by (auto simp: eval_nat_numeral)
   from c_sem have "c \<turnstile> (c,s(?CONT:=1))\<Rightarrow>\<^bsup>z\<^esup> t(?CONT:=1)"
     using fresh tnoninterference by (meson dual_order.refl)
-  
+
   hence "(translate ?CONT c, s(?CONT:=1)) \<Rightarrow>'\<^bsup> 5 + z\<^esup> t(?CONT := 0)"
     using translate_sound invar fresh by (fastforce simp: numeral_eq_Suc)
 
-  hence "(compile c,s)\<Rightarrow>'\<^bsup> 7 + z\<^esup> t(?CONT := 0)" unfolding compile_def 
+  hence "(compile c,s)\<Rightarrow>'\<^bsup> 7 + z\<^esup> t(?CONT := 0)" unfolding compile_def
     using 1 apply (simp add: numeral_eq_Suc)
-    by (smt (verit, best) IMP_Calls.Seq'' add_2_eq_Suc numeral_2_eq_2) 
-  
+    by (smt (verit, best) IMP_Calls.Seq'' add_2_eq_Suc numeral_2_eq_2)
+
   with that show ?thesis by simp
 qed
-  
 
-lemma compile_complete:
-  assumes sem: "(compile c,s) \<Rightarrow>'\<^bsup>7+z\<^esup> t"
+
+lemma compile_complete_add:
+  assumes sem: "(compile c,s) \<Rightarrow>'\<^bsup>z + 7\<^esup> t"
       and invar: "invar c"
   obtains t' where "c \<turnstile> (c,s)\<Rightarrow>\<^bsup>z\<^esup> t'" and "t = t' on set (vars c)"
 proof -
@@ -510,11 +510,31 @@ proof -
   hence "c \<turnstile> (c,s(?CONT:=1)) \<Rightarrow>\<^bsup>z\<^esup> t(?CONT:=1)"
     using translate_complete small_complete fresh invar by (fastforce simp: numeral_eq_Suc)
 
-  hence "c \<turnstile> (c,s) \<Rightarrow>\<^bsup>z\<^esup> t(?CONT:=s ?CONT)" 
+  hence "c \<turnstile> (c,s) \<Rightarrow>\<^bsup>z\<^esup> t(?CONT:=s ?CONT)"
     using tnoninterference[where S="set (vars c)"] fresh invar apply auto
     by (smt (verit, best) dual_order.refl fresh fun_upd_triv fun_upd_upd)
 
   with that show ?thesis using fresh by auto
 qed
+
+lemma compile_time_7_le:
+  assumes "(compile c,s) \<Rightarrow>'\<^bsup>z\<^esup> t"
+  shows "7 \<le> z"
+  using assms
+proof (induction "compile c" s z t arbitrary: c rule: big_step_t'_induct)
+case (Seq' c1 s1 x s2 c2 y s3 z)
+then show ?case
+  apply (auto simp: compile_def Let_def translate_def)
+  apply (erule While'_tE)
+  apply auto
+  done
+qed (auto simp: compile_def Let_def translate_def)
+
+lemma compile_complete:
+  assumes "(compile c,s) \<Rightarrow>'\<^bsup>z\<^esup> t"
+      and "invar c"
+  obtains t' where "c \<turnstile> (c,s)\<Rightarrow>\<^bsup>z - 7\<^esup> t'" and "t = t' on set (vars c)"
+  using assms compile_complete_add compile_time_7_le
+  by (metis add.commute le_add_diff_inverse)
 
 end
